impredicative_set/iparametricity_codensity.v
@@ -3,11 +3,7 @@
 From mathcomp Require Import all_ssreflect.
 From HB Require Import structures.
 Require Import ipreamble ihierarchy imonad_lib ifmt_lifting imonad_model.
-From elpi Require Import derive (*param2*).
-Require Import param1 param2.
-(*From elpi Require Import derive.std.*)
-(*From elpi Require Import derive.legacy.*)
-(*From elpi Require Import derive.experimental.*)
+From elpi Require Import derive param2.
 
 (**md**************************************************************************)
 (* Instantiations of uniform lifting (Theorem 27 of [Mauro Jaskelioff,        *)
@@ -72,82 +68,53 @@ Check uniform_sigma_lifting (M := [the monad of idfun]) _ _ Identity.naturality.
 
 Module Exception.
 Section exception_naturality.
-(*Variables Z A : UU0.
 
-Realizer Z as Z_R := (@eq Z).
-Realizer A as A_R := (@eq A).*)
-
-(*
-This typechecks:
-
-Inductive
-sum_R (A1 A2 : UU0) (A_R : A1 -> A2 -> UU0) (B1 B2 : UU0) (B_R : B1 -> B2 -> UU0)
-  : A1 + B1 -> A2 + B2 -> UU0 :=
-    inl_R : forall (_1 : A1) (_2 : A2), A_R _1 _2 -> sum_R (*A1 A2 A_R B1 B2 B_R*) (inl _1) (inl _2)
-  | inr_R : forall (_1 : B1) (_2 : B2), B_R _1 _2 -> sum_R (*A1 A2 A_R B1 B2 B_R*) (inr _1) (inr _2).
-*)
-
-#[verbose] derive sum.
-Print sum_R.
-(*
-coq-elpi creates sum_R at UU1, not UU0.
-Inductive
-sum_R (A1 A2 : UU1) (A_R : A1 -> A2 -> UU1) (B1 B2 : UU1) (B_R : B1 -> B2 -> UU1)
-  : A1 + B1 -> A2 + B2 -> UU1 :=
-    inl_R : forall (_1 : A1) (_2 : A2), A_R _1 _2 -> sum_R A1 A2 A_R B1 B2 B_R (inl _1) (inl _2)
-  | inr_R : forall (_1 : B1) (_2 : B2), B_R _1 _2 -> sum_R A1 A2 A_R B1 B2 B_R (inr _1) (inr _2).
-*)
-
-#[verbose] derive ExceptMonad.acto.
-Fail Elpi derive.param2 ExceptMonad.acto.
-
-(*
-sum_R at UU1 causes a universe inconsistency:
-
-Error:
-param2: constant does not have the right type: Unable to unify
- "forall E1 E2 : UU0,
-  (E1 -> E2 -> UU0) ->
-  forall A1 A2 : UU0, (A1 -> A2 -> UU0) -> E1 + A1 -> E2 + A2 -> UU1"
-with
- "forall E1 E2 : UU0,
-  (E1 -> E2 -> UU0) ->
-  forall A1 A2 : UU0,
-  (A1 -> A2 -> UU0) -> ExceptMonad.acto E1 A1 -> ExceptMonad.acto E2 A2 -> UU0"
-(universe inconsistency: Cannot enforce sum_R.u0 <= Set).
-*)
-
-derive eq.
-
-Definition M (Z : UU0) := ExceptMonad.acto Z.
-(*Definition M (Z : UU0) : monad := ExceptMonad.acto Z.*)
-
-derive M.
+Let M (Z : UU0) := ExceptMonad.acto Z.
+(* Bad: `Definition M (Z : UU0) : monad := ExceptMonad.acto Z.`
+   Annotating `M Z` to be of type `monad` inserts a reverse coercion,
+   which blocks
+   `derive M` and hence `#[recursive] derive T`.
+   More precisely, reverse coercions contain a constant `ReverseCoercionSource`
+   that is both universe polymorphic and global, which cannot be handled by
+   `coq-elpi`.
+ *)
 
 Definition Me (Z : UU0) (X : UU0) : UU0 := ltac:(
   let t := constr:(M Z X) in
   let t := eval cbn in t in
   exact t).
 
-derive Me.
-
 Definition T (Z A : UU0) : UU0 := MK (Me Z) A.
 
-(*Parametricity Recursive T arity 2.*)
+(* In order to derive `param2` on `ExceptMonad.acto`,
+   we cannot use `Datatypes.sum` in its definition.
+   `Datatypes.sum` is defined with template universe polymorphism,
+   which means, syntactically, its universe is set to `Type`,
+   while our instance of `sum` (in `ExceptMonad.acto`) will reside in `Set`.
+   `coq-elpi` supposedly analyzes the definition of `sum` via its syntax,
+   and generates `sum_R` in `Type` (= `UU1`), resulting in a
+   universe inconsistency when doing `Elpi derive.param2 ExceptMonad.acto`.
+   We have redefined `sum` in `imonad_model.v` explicitly
+   in `Set` to avoid this problem. *)
 
-#[verbose] derive MK.
 #[recursive] derive T.
+(* This automatically does:
+Elpi derive.param2 ExceptMonad.acto.
+Elpi derive.param2 M.
+Elpi derive.param2 Me.
+Elpi derive.param2 MK.
+and more. *)
 
 Variables Z A : UU0.
 Variable m : T Z A.
 
-Axiom param : T_R _ _ (@eq Z) m m.
+Axiom param : T_R Z Z (@eq Z) A A (@eq A) m m.
 
-Lemma naturality : naturality (exponentialF A \o M) M m.
+Lemma naturality : naturality (exponentialF A \o (M Z)) (M Z) m.
 Proof.
 move=> X Y f; apply funext => eX.
 set rhs := RHS.
-have : Me_R X Y (fun x y => f x = y) (m X eX) rhs.
+have : Me_R _ _ (@eq Z) X Y (fun x y => f x = y) (m X eX) rhs.
   apply: param => a _ <-; rewrite Actm_exponenialFE compE.
   by case: (eX a) => [e|x]; constructor.
 by rewrite compE; case=> [a _ <-|x _ <-].
@@ -180,27 +147,27 @@ Check uniform_sigma_lifting (M := [the monad of option_monad]) _ _ Option.natura
 (******************************************************************************)
 
 Module List.
+Import IListMonad.
 Section list_naturality.
-Variable A : UU0.
 
-Realizer A as A_R := (@eq A).
-
-Let M := [the monad of ListMonad.acto].
+Let M : UU0 -> UU0 := seq.
+Let MM := [the monad of IListMonad.acto].
+Lemma MME : MM = M :> (_ -> _). Proof. by []. Qed.
 
 Definition Ml (X : UU0) : UU0 := ltac:(
   let t := constr:(M X) in
   let t := eval cbn in t in
   exact t).
 
-Definition T : UU0 := MK Ml A.
+Definition T (A : UU0) : UU0 := MK Ml A.
 
-Parametricity Recursive T arity 2.
+#[recursive] derive T.
 
-Variable m : T.
+Variable A : UU0.
+Variable m : T A.
+Axiom param : T_R A A (@eq A) m m.
 
-Axiom param : T_R m m.
-
-Lemma naturality : naturality (exponentialF A \o M) M m.
+Lemma naturality : naturality (exponentialF A \o MM) MM m.
 Proof.
 move=> X Y f /=; apply funext => eX.
 set rhs := RHS.
@@ -211,58 +178,60 @@ by rewrite compE; elim => // x _ <- l _ _ <-.
 Qed.
 
 End list_naturality.
-End List.
 
-Check uniform_sigma_lifting (M := [the monad of ListMonad.acto]) _ _ List.naturality.
+Check uniform_sigma_lifting (M := [the monad of IListMonad.acto]) _ _ List.naturality.
+
+End List.
 
 (******************************************************************************)
 
 Module State.
+Import IStateMonad.
 Section state_naturality.
-Variable S A : UU0.
 
-Realizer S as S_R := (@eq S).
-Realizer A as A_R := (@eq A).
+Let M (S : UU0) := IStateMonad.acto S.
+Let MM (S : UU0) := [the monad of IStateMonad.acto S].
+Lemma MME : MM = M :> (_ -> _). Proof. by []. Qed.
 
-Let M := [the monad of StateMonad.acto S].
-
-Definition Ms X : UU0 := ltac:(
-  let t := constr:(M X) in
+Definition Ms (S X : UU0) := ltac:(
+  let t := constr:(M S X) in
   let t := eval cbn in t in
   exact t).
 
-Definition T : UU0 := MK Ms A.
+Definition T (S A : UU0) : UU0 := MK (Ms S) A.
 
-Parametricity Recursive T arity 2.
+#[recursive] derive T.
 
-Variable m : T.
+Variable S A : UU0.
+Variable m : T S A.
 
-Axiom param : T_R m m.
+Axiom param : T_R S S (@eq S) A A (@eq A) m m.
 
-Lemma Actm_ModelMonadStateE' (X Y : UU0) (f : X -> Y) (eX : (exponentialF A \o M) X) a (s : S):
-  (M # f \o eX) a s = let (x, y) := eX a s in (f x, y).
+Lemma Actm_ModelMonadStateE' (X Y : UU0) (f : X -> Y) (eX : (exponentialF A \o MM S) X) a (s : S):
+  (MM S # f \o eX) a s = let (x, y) := eX a s in (f x, y).
 Proof. by []. Qed.
 
 Lemma Actm_ModelMonadStateE (X Y : UU0) (f : X -> Y) (eX : A -> S -> (X * S)) (s : S)
-  (mX : (A -> Ms X) -> Ms X) :
-  (M # f \o mX) eX s = (let (x, y) := mX eX s in (f x, y)).
+  (mX : (A -> Ms S X) -> Ms S X) :
+  (MM S # f \o mX) eX s = (let (x, y) := mX eX s in (f x, y)).
 Proof. by []. Qed.
 
-Lemma naturality : naturality (exponentialF A \o M) M m.
+Lemma naturality : naturality (exponentialF A \o MM S) (MM S) m.
 Proof.
 move=> X Y f; apply funext => eX.
 set rhs := RHS.
-have H : Ms_R X Y (fun x y => f x = y) (m X eX) rhs.
-  apply param => // a _ <- s1 _ <-.
+have H : Ms_R _ _ (@eq S) X Y (fun x y => f x = y) (m X eX) rhs.
+  apply: param => // a _ <- s1 _ <-.
   rewrite Actm_exponenialFE Actm_ModelMonadStateE'.
-  by case: (eX a) => x s2; exact: prod_R_pair_R.
+  by case: (eX a) => x s2; exact: pair_R.
 apply funext => s.
-have {}H : prod_R X Y (fun x y => f x = y) S S S_R (m X eX s) (rhs s) by exact: H.
+have {}H : prod_R X Y (fun x y => f x = y) S S (@eq S) (m X eX s) (rhs s) by exact: H.
 inversion H as [x y fxy s1 s2 s12 xs1 ys2].
 by rewrite Actm_ModelMonadStateE -xs1 fxy s12.
 Qed.
 End state_naturality.
-End State.
 
 Check fun S => uniform_sigma_lifting
-  (M := [the monad of StateMonad.acto S]) _ _ (State.naturality S).
+  (M := [the monad of IStateMonad.acto S]) _ _ (State.naturality S).
+
+End State.
